src/Parsers/BooleanRecognizer.v
@@ -101,30 +101,32 @@ Section recursive_descent_parser.
           : bool.
           Proof.
             refine
-              (sumbool_rect
-                 (fun _ => bool)
-                 (fun _ => (** [str] got smaller, so we reset the valid nonterminals list *)
-                    parse_productions
-                      (@parse_nonterminal
+              (parse_productions
+                 (sumbool_rect
+                    (fun b => forall (str' : String), str' ≤s (if b then str else str0) -> String.string -> bool)
+                    (fun _ => (** [str] got smaller, so we reset the valid nonterminals list *)
+                       @parse_nonterminal
                          (str : String, initial_nonterminals_data)
                          (or_introl _))
-                      (or_intror (reflexivity _))
-                      (Lookup G nt))
-                 (fun _ => (** [str] didn't get smaller, so we cache the fact that we've hit this nonterminal already *)
-                    sumbool_rect
-                      (fun _ => bool)
-                      (fun _ => (** It was valid, so we can remove it *)
-                         parse_productions
-                           (@parse_nonterminal
+                    (fun _ => (** [str] didn't get smaller, so we cache the fact that we've hit this nonterminal already *)
+                       sumbool_rect
+                         (fun _ => forall (str' : String), str' ≤s str0 -> String.string -> bool)
+                         (fun _ => (** It was valid, so we can remove it *)
+                            @parse_nonterminal
                               (str0 : String, remove_nonterminal valid nt)
                               (or_intror (conj eq_refl (remove_nonterminal_dec _ nt _))))
-                           (str := str)
-                           _
-                           (Lookup G nt))
-                      (fun _ => (** oops, we already saw this nonterminal in the past.  ABORT! *)
-                         false)
-                      (Sumbool.sumbool_of_bool (is_valid_nonterminal valid nt)))
-                 (lt_dec (length str) (length str0)));
+
+                         (fun _ _ _ _ => (** oops, we already saw this nonterminal in the past.  ABORT! *)
+                            false)
+                         (Sumbool.sumbool_of_bool (is_valid_nonterminal valid nt)))
+                    (lt_dec (length str) (length str0)))
+                 (str := str)
+                 (sumbool_rect
+                    (fun b => str ≤s (if b then str else str0))
+                    (fun _ => or_intror (reflexivity _))
+                    (fun _ => _)
+                    (lt_dec (length str) (length str0)))
+                 (Lookup G nt));
             assumption.
           Defined.
         End step.
