src/Parsers/BooleanRecognizerOptimized.v
@@ -38,65 +38,11 @@ Proof.
   destruct a; trivial.
 Qed.
 
-Ltac Fix3_setoid_rewrite H :=
-  etransitivity;
-  [ try clear H
-  | match goal with
-      | [ |- _ = @Fix ?A ?R ?Rwf (fun a : ?A => forall (b :@?B a) (c : @?C a b) (d : @?D a b c), @?P a b c d) ?f ?a ?b ?c ?d ]
-        => refine ((fun H => @Fix3_Proper_eq A B C D R Rwf P _ f H a b c d) _)
-    end;
-    unfold forall_relation, pointwise_relation, respectful;
-    let H' := fresh in
-    (intros ??? H' ???);
-      let L := match goal with |- ?L = _ => constr:L end in
-      let e := fresh "e" in
-      set (e := L);
-        setoid_rewrite <- (parse_production_respectful H');
-        setoid_rewrite H; try clear H;
-        subst e;
-        reflexivity ].
-
-Ltac extract_parser_opt :=
-  eexists;
-  let L := match goal with |- ?L = _ => constr:L end in
-  let e := fresh "e" in
-  set (e := L);
-  let G := match goal with |- _ = parse_nonterminal (G := ?G) _ _ => constr:G end in
-  let G' := head G in
-  try unfold G';
-    cbv beta iota zeta delta [parse_nonterminal parse_nonterminal_or_abort parse_nonterminal_step parse_productions parse_item Lookup list_to_grammar list_to_productions];
-    simpl;
-    repeat Fix3_setoid_rewrite (fun ls => eq_sym (@fold_symmetric _ orb Bool.orb_assoc Bool.orb_comm false ls));
-    repeat
-      (let H0 := fresh "H0" in
-       match goal with
-         | [ |- context[fold_right ?f ?i (map _ (bool_rect _ ?x ?y (string_beq ?s _)))] ]
-           => (pose proof (fun g s' => @pull_bool_rect _ _ (fun ls => fold_right f i (map g ls)) x y (string_beq s s')) as H0;
-               simpl in H0;
-               Fix3_setoid_rewrite H0)
-         | [ |- appcontext[fold_right (fun str_t else_case s => bool_rect (fun _ => ?T) (@?a str_t) (else_case s) (@?b str_t s))] ]
-           => (pose proof (@fold_right_fun _ _ _ (fun str_t else_cases s => bool_rect (fun _ => T) (a str_t) else_cases (b str_t s))) as H0;
-               simpl in H0;
-               Fix3_setoid_rewrite H0)
-         | [ |- context[@map _ ?B _ (fold_right (fun x acc => bool_rect (fun _ => _) (@?a x) acc _) ?init ?ls)] ]
-           => (pose proof (fun b' f => @f_fold_right_bool_rect _ (list B) _ (map f) init ls a b') as H0;
-               simpl in H0;
-               Fix3_setoid_rewrite H0)
-         | [ |- appcontext[?f (fold_right (fun x acc => bool_rect (fun _ => _) _ acc _) _ ?ls) ?x] ]
-           => (pose proof (fun init => @f_fold_right_bool_rect _ _ _ (fun k => f k x) init ls) as H0;
-               simpl in H0;
-               Fix3_setoid_rewrite H0)
-         | [ |- appcontext[?f (fold_right (fun x acc => bool_rect (fun _ => _) _ acc _) _ ?ls)] ]
-           => (pose proof (fun init => @f_fold_right_bool_rect _ _ _ f init ls) as H0;
-               simpl in H0;
-               Fix3_setoid_rewrite H0)
-       end;
-       instantiate;
-       simpl);
-    repeat Fix3_setoid_rewrite Bool.orb_false_r;
-    subst e;
-    cbv beta iota zeta delta [bool_rect sumbool_rect];
-    reflexivity.
+Local Ltac simpl_setoid_rewrite lem :=
+  let H := fresh in
+  pose proof lem as H;
+    setoid_rewrite H;
+    clear H.
 
 Section recursive_descent_parser.
   Context {Char} {HSL : StringLike Char} {HSLP : StringLikeProperties Char}
@@ -109,6 +55,66 @@ Section recursive_descent_parser.
              (nt : String.string)
   : { b : bool | b = parse_nonterminal (G := G) str nt }.
   Proof.
-    extract_parser_opt.
+    let G := match goal with |- context[_ = parse_nonterminal (G := ?G) _ _] => constr:G end in
+    let G' := head G in
+    try unfold G';
+      cbv beta iota zeta delta [parse_nonterminal parse_nonterminal_or_abort parse_nonterminal_step parse_productions parse_item Lookup list_to_grammar list_to_productions];
+      simpl;
+      eexists;
+      let L := match goal with |- ?L = _ => constr:L end in
+      let e := fresh "e" in
+      let e' := fresh "e" in
+      let pp := fresh "pp" in
+      set (e := L);
+        etransitivity;
+        [
+        | match goal with
+            | [ |- _ = @Fix ?A ?R ?Rwf (fun a : ?A => forall (b :@?B a) (c : @?C a b) (d : @?D a b c), @?P a b c d) ?f ?a ?b ?c ?d ]
+              => refine ((fun H => @Fix3_Proper_eq A B C D R Rwf P _ f H a b c d) _)
+          end;
+          unfold forall_relation, pointwise_relation, respectful;
+          let H' := fresh in
+          (intros ??? H' ???);
+            let L := match goal with |- ?L = ?R => constr:L end in
+            let R := match goal with |- ?L = ?R => constr:R end in
+            set (e' := L);
+              let R' := match type of H' with
+                          | forall a0 a1 a2 a3 a4, ?x a0 a1 a2 a3 a4 = ?y a0 a1 a2 a3 a4
+                            => let Rp := (eval pattern y in R) in
+                               match Rp with
+                                 | ?R' y => (eval cbv beta in (R' x))
+                               end
+                        end in
+              transitivity R';
+                [ clear H';
+                  match goal with
+                    | [ |- appcontext[@parse_production ?a ?b ?c ?d ?e ?f ?g ?h] ]
+                      => set (pp := @parse_production a b c d e f g h)
+                  end
+                | clear -H'; unfold sumbool_rect;
+                  repeat match goal with
+                           | _ => reflexivity
+                           | [ |- appcontext[match ?e with left _ => _ | right _ => _ end] ]
+                             => destruct e
+                         end;
+                  setoid_rewrite (parse_production_respectful H');
+                  reflexivity ] ];
+        [
+        | repeat match goal with
+                   | _ => progress simpl
+                   | _ => setoid_rewrite (fun ls => eq_sym (@fold_symmetric _ orb Bool.orb_assoc Bool.orb_comm false ls))
+                   | _ => setoid_rewrite Bool.orb_false_r
+                   | [ |- appcontext[fold_right (fun str_t else_case s => bool_rect (fun _ => ?T) (@?a str_t) (else_case s) (@?b str_t s))] ]
+                     => simpl_setoid_rewrite (@fold_right_fun _ _ _ (fun str_t else_cases s => bool_rect (fun _ => T) (a str_t) else_cases (b str_t s)))
+                   | [ |- appcontext[?f (fold_right (fun x acc => bool_rect (fun _ => _) _ acc _) _ ?ls) ?x] ]
+                     => simpl_setoid_rewrite (fun init => @f_fold_right_bool_rect _ _ _ (fun k => f k x) init ls)
+                   | [ |- appcontext[?f (fold_right (fun x acc => bool_rect (fun _ => _) _ acc _) _ ?ls)] ]
+                     => simpl_setoid_rewrite (fun init => @f_fold_right_bool_rect _ _ _ f init ls)
+                 end;
+          subst pp; simpl;
+          subst e'; instantiate; reflexivity ];
+        cbv beta iota zeta delta [bool_rect sumbool_rect];
+        subst e; instantiate.
+    reflexivity.
   Defined.
 End recursive_descent_parser.
